backend/Reloadtyping.v
@@ -288,16 +288,13 @@ Proof.
     rewrite loc_arguments_type; auto.
   destruct ros. destruct H2 as [A [B C]]. auto 10 with reloadty. 
   auto 10 with reloadty.
-
-  destruct (ef_reloads ef) as [] eqn:?.
+  destruct (ef_reloads ef) eqn:?.
   assert (arity_ok (sig_args (ef_sig ef)) = true) by intuition congruence.
   assert (map mreg_type (regs_for args) = map Loc.type args).
     apply wt_regs_for. apply arity_ok_enough. congruence.
   assert (mreg_type (reg_for res) = Loc.type res). eauto with reloadty.
   auto 10 with reloadty.
   auto with reloadty.
-
-
 
   assert (map mreg_type (regs_for args) = map Loc.type args).
     eauto with reloadty.
