cfrontend/Initializersproof.v
@@ -380,6 +380,13 @@ Proof.
   eelim Mem.perm_empty; eauto. 
 Qed.
 
+Lemma mem_empty_not_weak_valid_pointer:
+  forall b ofs, Mem.weak_valid_pointer Mem.empty b ofs = false.
+Proof.
+  intros. unfold Mem.weak_valid_pointer.
+  now rewrite !mem_empty_not_valid_pointer.
+Qed.
+
 Lemma sem_cmp_match:
   forall c v1 ty1 v2 ty2 m v v1' v2' v',
   sem_cmp c v1 ty1 v2 ty2 Mem.empty = Some v ->
@@ -391,10 +398,12 @@ Opaque zeq.
   intros. unfold sem_cmp in *.
   destruct (classify_cmp ty1 ty2); try (destruct s); inv H1; inv H2; inv H; inv H0; auto with mval.
   destruct (Int.eq n Int.zero); try discriminate. 
-  unfold sem_cmp_mismatch in *. destruct c; inv H3; inv H2; constructor.
+  unfold Val.cmp_different_blocks in *. destruct c; inv H3; inv H2; constructor.
   destruct (Int.eq n Int.zero); try discriminate. 
-  unfold sem_cmp_mismatch in *. destruct c; inv H2; inv H1; constructor.
-  rewrite (mem_empty_not_valid_pointer (Zpos id) (Int.unsigned ofs)) in H4. discriminate.
+  unfold Val.cmp_different_blocks in *. destruct c; inv H2; inv H1; constructor.
+  rewrite (mem_empty_not_valid_pointer (Zpos id) (Int.unsigned ofs)) in H4.
+  rewrite (mem_empty_not_weak_valid_pointer (Zpos id) (Int.unsigned ofs)) in H4. simpl in H4.
+  destruct (zeq (Z.pos id) (Z.pos id0)); discriminate.
 Qed.
 
 Lemma sem_binary_match:
